Finish conversion from separation logic to statically-known state-space

AttarchProperties.v
@@ -3,11 +3,9 @@ Require Import Ctl.Definition.
 Require Import Ctl.Tactics.
 Require Import Ctl.Properties.
 
-Require Import SepLogic.Definition.
-Require Import SepLogic.Entailment.
-
 Require Import BinaryRelations.
 Require Import TransitionSystems.
+Require Import Privilege.
 Require Import AttarchTrans.
 
 Require Import Coq.Program.Equality.
@@ -15,37 +13,27 @@ Require Import Coq.Relations.Relation_Definitions.
 Require Import Coq.Relations.Relation_Operators.
 Require Import GeneralTactics.
 
-(* Assert some fact about the global state *)
-Definition gassert {comp loc L} (s: sprop comp loc) : TProp (sprop comp loc * L) :=
-    TLift (fun st => exists frame, fst st ⊢ s ** frame).
+Definition useram_key_secure := 
+  ⟨fun (st: attarch_global * attarch_state) =>
+    val_at (useram_key (fst st)) = Some good_useram_key -> 
+    acc_at (useram_key (fst st)) = useram_key_acc
+  ⟩. 
 
-Theorem useram_key_never_compromised: forall V (v: V) (acc: access component),
-  acc malicious_linux_component read ->
-  attarch_strans; (⟨⟩, boot_from_good_plat) ⊨ ¬ EF (gassert (useram_key #acc ↦ v)).
+Theorem useram_key_never_compromised:
+  attarch_trans @initial_state_good ⊨ AG useram_key_secure.
 Proof.
-  intros V v acc Hmal_acc.
-  tapply AG_EF.
   apply rtc_AG.
   intros s' Hsteps.
   dependent induction Hsteps.
-  - simpl. 
-    (* Trivial by sentails discrimination *)
-    admit.
-  - 
-    (* intros Hcontra. *)
-    invc H.
-    invc H2.
-    + intro Hcontra.
-      simpl in Hcontra.
-      (* Hcontra is a contradiction. 
-         y' can only entail `bootev # readonly ↦ ...`, by H1.
-         z0 can't entail `useram_key # ...` either, by IHHsteps
-       *)
-      admit.
-    + (* Hsteps is an impossible path *)
-      invc Hsteps.
-      invc H.
-      inv H9.
-    +  
-
-Admitted.
+  - discriminate.
+  - invc H.
+    + apply IHHsteps.
+    + invc H0.
+      * invc H1.
+       -- apply IHHsteps.
+       -- apply IHHsteps.
+       -- simpl. reflexivity.
+      * invc H1.
+       -- apply IHHsteps.
+       -- invc H0; apply IHHsteps.
+Qed.
