AttarchTrans.v
@@ -10,7 +10,12 @@ Inductive component : Set :=
   | useram
   | malicious_linux_component.
 
-Definition mem_store v : Type := access component * v.
+Record mem_store v : Type := mkMem_store 
+  { acc_at: access component
+  ; val_at: option v
+  }.
+Arguments acc_at {v}%type_scope.
+Arguments val_at {v}%type_scope.
 
 Record attarch_global := mkAttarchGl
   { boot_ev    : mem_store nat
@@ -18,7 +23,29 @@ Record attarch_global := mkAttarchGl
   ; useram_key : mem_store nat
   }.
 
-Definition stransition a := transition (sprop component loc) a.
+Definition set_boot_ev (st: attarch_global) (m: mem_store nat) : attarch_global :=
+  {| boot_ev    := m; 
+     vm_ev      := vm_ev st;
+     useram_key := useram_key st |}.
+Definition set_vm_ev (st: attarch_global) (m: mem_store nat) : attarch_global :=
+  {| boot_ev    := boot_ev st;
+     vm_ev      := m;
+     useram_key := useram_key st |}.
+Definition set_useram_key (st: attarch_global) (m: mem_store nat) : attarch_global :=
+  {| boot_ev    := boot_ev st; 
+     vm_ev      := vm_ev st;
+     useram_key := m |}.
+
+Definition good_boot_ev : nat.
+exact 0. Qed.
+Definition bad_boot_ev  : nat.
+exact 0. Qed.
+Definition initial_global_state_good :=
+  {| boot_ev    := {|acc_at := allAcc; val_at := Some good_boot_ev|};
+     vm_ev      := {|acc_at := allAcc; val_at := None|};
+     useram_key := {|acc_at := allAcc; val_at := None|}
+  |}.
+
 
 (* Add linux state under vm? *)
 (* Note, all sudoers have access to useram/platam channel *)
@@ -29,13 +56,13 @@ Inductive useram_state : Set :=
   | useram_making_request
   | useram_sending_response.
 
-Inductive useram_trans : stransition useram_state :=
-  | useram_get_key : forall (acc: access component) (k: nat),
-      acc useram read ->
-      useram_trans
-        (useram_key #acc ↦ k, useram_waiting_key)
-        (useram_key #acc ↦ k, useram_waiting_request)
-  (* | useram_get_request : useram_trans 
+Inductive useram_trans : transition attarch_global useram_state :=
+  | useram_get_key : forall st,
+      acc_at (useram_key st) useram read ->
+      useram_trans 
+        (st, useram_waiting_key)
+        (st, useram_waiting_request)
+ (* | useram_get_request : useram_trans 
       (s, useram_waiting_key)
       (s,useram_) *)
   .
@@ -48,58 +75,62 @@ Inductive platam_state : Set :=
 
 Definition good_vm_ev : nat. Admitted.
 Definition bad_vm_ev  : nat. Admitted.
-Definition useram_key_val  : nat. Admitted.
+Definition good_useram_key : nat. Admitted.
 Inductive useram_key_acc : access component :=
   | useram_useram_key_read  : useram_key_acc useram read
   | platam_useram_key_read  : useram_key_acc platam read
   | platam_useram_key_write : useram_key_acc platam write.
-Inductive platam_trans : stransition platam_state :=
-  | platam_measure_good_vm : platam_trans
-      (⟨⟩, platam_init)
-      (vm_ev #private platam ↦ good_vm_ev, platam_appraise)
-  | platam_measure_bad_vm : platam_trans
-      (⟨⟩, platam_init)
-      (vm_ev #private platam ↦ bad_vm_ev, platam_appraise)
-  | platam_release_key : forall (acc: access component),
-      acc platam read ->
+
+Inductive platam_trans : transition attarch_global platam_state :=
+  | platam_measure_good_vm : forall st,
       platam_trans
-        (vm_ev #acc ↦ good_vm_ev,
-          platam_appraise)
-        (vm_ev #acc ↦ good_vm_ev **
-        useram_key #useram_key_acc ↦ useram_key_val,
-          platam_run).
+        (st, platam_init)
+        (set_vm_ev st {|acc_at := private platam; val_at := Some good_vm_ev|}, platam_appraise)
+  | platam_measure_bad_vm : forall st,
+      platam_trans
+        (st, platam_init)
+        (set_vm_ev st {|acc_at := private platam; val_at := Some bad_vm_ev|}, platam_appraise)
+  | platam_release_key : forall st,
+      acc_at (vm_ev st) platam read ->
+      val_at (vm_ev st) = Some good_vm_ev ->
+      platam_trans
+        (st, platam_appraise)
+        (set_useram_key st {|acc_at := useram_key_acc; val_at := Some good_useram_key|}, platam_run).
 
 Inductive vm_state : Set :=
   | vm_init
   | vm_run : useram_state -> vm_state.
 
-Inductive vm_trans : stransition vm_state :=
-  | vm_boot : vm_trans
-      (⟨⟩, vm_init)
-      (⟨⟩, vm_run useram_waiting_key)
+Inductive vm_trans : transition attarch_global vm_state :=
+  | vm_boot : forall st,
+      vm_trans 
+        (st, vm_init)
+        (st, vm_run useram_waiting_key)
   | vm_linux_step : forall g g' s s',
       useram_trans (g,s) (g',s') ->
       vm_trans
         (g, vm_run s)
-        (g, vm_run s').
+        (g', vm_run s').
 
 Inductive attarch_state : Set :=
-  | boot_from_good_plat (* initial state *)
-  | boot_from_bad_plat  (* initial state *)
+  | boot
   | sel4_run : platam_state * vm_state -> attarch_state.
 
-Definition good_boot_ev : nat. Admitted.
-Definition bad_boot_ev  : nat. Admitted.
-Inductive attarch_trans : stransition attarch_state :=
-  | good_boot : attarch_trans 
-      (⟨⟩, boot_from_good_plat)
-      (boot_ev #readonly ↦ good_boot_ev, sel4_run (platam_init, vm_init))
-  | bad_boot : attarch_trans 
-      (⟨⟩, boot_from_bad_plat)
-      (boot_ev #readonly ↦ bad_boot_ev, sel4_run (platam_init, vm_init))
+Inductive attarch_trans : transition attarch_global attarch_state :=
+  (* | good_boot : forall st,
+      (fst (boot_ev st)) sel4 read ->
+      (snd (boot_ev st)) = good_boot_ev ->
+      attarch_trans 
+        (st, boot_from_good_plat)
+        (st, sel4_run (platam_init, vm_init)) *)
+  | attarch_boot : forall st,
+      attarch_trans 
+        (st, boot)
+        (st, sel4_run (platam_init, vm_init))
   | component_step : forall g g' s s',
       (platam_trans ⊔ vm_trans) (g,s) (g',s') ->
       attarch_trans 
         (g, sel4_run s)
         (g', sel4_run s').
-Definition attarch_strans := sentails_clos attarch_trans.
+
+Definition initial_state_good := (initial_global_state_good, boot).
