Ctl/Definition.v
@@ -38,7 +38,7 @@ Arguments EU    {state}%type_scope.
 
 Notation "⊤" := (TTop).
 Notation "⊥" := (TBot).
-(* Notation "⟨ P ⟩" := (TLift P) (at level 35). *)
+Notation "⟨ P ⟩" := (TLift P) (at level 35, format "⟨ P ⟩").
 Notation "P ∧ Q" := (TConj P Q) (at level 45, right associativity).
 Notation "P ∨ Q" := (TDisj P Q) (at level 55, right associativity).
 Notation "P --> Q" := (TImpl P Q) (at level 68,  right associativity).
@@ -47,26 +47,26 @@ Notation "¬ P" := (TNot P) (at level 40).
 Notation "'A' [ P 'U' Q ]" := (AU P Q) (at level 40).
 Notation "'E' [ P 'U' Q ]" := (EU P Q) (at level 40).
 
-Reserved Notation "M @ s ⊨ P" (at level 70, format "M @ s  ⊨  P").
-Reserved Notation "M @ s ⊭ P" (at level 70, format "M @ s  ⊭  P").
+Reserved Notation "M @ s ⊨ P" (at level 70, format "M  @ s  ⊨  P").
+Reserved Notation "M @ s ⊭ P" (at level 70, format "M  @ s  ⊭  P").
 (* Replace binary_relation with serial_transition if needed *)
 Fixpoint tEntails {state} (R: relation state) (s: state) (tp: TProp state) : Prop :=
   match tp with
   | ⊤ => True
   | ⊥ => False
-  | TLift P => P s
-  | ¬P => R@s ⊭ P
-  | P ∧ Q => R@s ⊨ P /\ R@s ⊨ Q
-  | P ∨ Q => R@s ⊨ P \/ R@s ⊨ Q
-  | P --> Q => R@s ⊨ P -> R@s ⊨ Q
-  | AX P => forall s', R s s' -> R@s' ⊨ P
-  | EX P => exists s', R s s' -> R@s' ⊨ P
-  | AG P => forall n, forall (p: path R s n), forall s', in_path s' p -> R@s' ⊨ P
-  | EG P => forall n, exists (p: path R s n), forall s', in_path s' p -> R@s' ⊨ P
-  | AF P => exists n, forall (p: path R s n), exists s', in_path s' p /\ R@s' ⊨ P
-  | EF P => exists n, exists (p: path R s n), exists s', in_path s' p /\ R@s' ⊨ P
+  | ⟨P⟩ => P s
+  | ¬P => R @s ⊭ P
+  | P ∧ Q => R @s ⊨ P /\ R @s ⊨ Q
+  | P ∨ Q => R @s ⊨ P \/ R @s ⊨ Q
+  | P --> Q => R @s ⊨ P -> R @s ⊨ Q
+  | AX P => forall s', R s s' -> R @s' ⊨ P
+  | EX P => exists s', R s s' -> R @s' ⊨ P
+  | AG P => forall n, forall (p: path R s n), forall s', in_path s' p -> R @s' ⊨ P
+  | EG P => forall n, exists (p: path R s n), forall s', in_path s' p -> R @s' ⊨ P
+  | AF P => exists n, forall (p: path R s n), exists s', in_path s' p /\ R @s' ⊨ P
+  | EF P => exists n, exists (p: path R s n), exists s', in_path s' p /\ R @s' ⊨ P
   (* TODO: AU and EU *)
   | _ => False
   end
   where "M @ s ⊨ P" := (tEntails M s P)
-    and "M @ s ⊭ P" := (~ M@s ⊨ P).
+    and "M @ s ⊭ P" := (~ M @s ⊨ P).
